define PCM for Atom

src/tlogic/TemporalLogic.v
@@ -1,7 +1,7 @@
 From stdpp Require Import coPset gmap namespaces.
 From sflib Require Import sflib.
 From Fairness Require Import PCM IProp IPM.
-From Fairness Require Import IndexedInvariants LogicSyntaxHOAS.
+From Fairness Require Import IndexedInvariants LogicSyntaxHOAS PCMForSyntax.
 From iris Require Import bi.big_op.
 From iris Require base_logic.lib.invariants.
 
@@ -52,16 +52,20 @@ Local Notation index := nat.
 
 (* End Base. *)
 
-Module Atoms.
+Module Atom.
 
   Section ATOMS.
 
     (* Context `{T : Type}. *)
 
+    Context `{σ : list PCMForSyntax.URA.t}.
+
     (* TODO: more atoms *)
 
-    (* Atoms do not interpret arguments. *)
+    (* Atom do not interpret arguments. *)
     Inductive t {Typ : Syntax.type -> Type} : Type :=
+    | own {M : PCMForSyntax.URA.t} {IN : In M σ} (r : M)
+    (* | own {M : PCMForSyntax.URA.t} {IN : PCMForSyntax.GRA.inG M σ} (r : M) *)
     | owne (E : coPset)
     | ownd (D : gset positive)
     | owni (i : positive) (p : @Syntax.t Typ (@t Typ))
@@ -83,21 +87,29 @@ Module Atoms.
 
   Section INTERP.
 
-    Context `{Σ : GRA.t}.
+    Context `{σ : list PCMForSyntax.URA.t}.
+    (* Local Notation σ := (PCMForSyntax.GRA.of_list _σ). *)
+    (* Context `{σ : PCMForSyntax.GRA.t}. *)
+    Context `{Σ : PCM.GRA.t}.
     (* Context `{T : Type}. *)
     (* Context `{TSem : T -> Type}. *)
+    Context `{SUB : forall M, In M σ -> PCM.GRA.inG (to_LURA M) Σ}.
 
-    Local Notation typing := (@Syntax.Typ (@t)).
-    Local Notation Formulas := (fun (i : index) => @Syntax.t (typing i) (@t (typing i))).
+    (* This is too strong. *)
+    (* Context `{SUB : forall (M : URA.t), PCMForSyntax.GRA.inG M σ -> PCM.GRA.inG (to_LURA M) Σ}. *)
+
+    Local Notation typing := (@Syntax.Typ (@t σ)).
+    Local Notation Formulas := (fun (i : index) => @Syntax.t (typing i) (@t σ (typing i))).
     (* Local Notation typing := (@Syntax.Typ T TSem (@t T)). *)
     (* Local Notation Formulas := (fun (i : index) => @Syntax.t T (typing i) (@t T (typing i))). *)
 
-    Context `{@GRA.inG (IInvSetRA Formulas) Σ}.
-    Context `{@GRA.inG (index ==> CoPset.t)%ra Σ}.
-    Context `{@GRA.inG (index ==> Gset.t)%ra Σ}.
+    Context `{@PCM.GRA.inG (IInvSetRA Formulas) Σ}.
+    Context `{@PCM.GRA.inG (PCM.URA.pointwise index PCM.CoPset.t) Σ}.
+    Context `{@PCM.GRA.inG (PCM.URA.pointwise index PCM.Gset.t) Σ}.
 
-    Definition to_semantics (n : index) (a : @t (typing n)) : iProp :=
+    Definition to_semantics (n : index) (a : @t σ (typing n)) : iProp :=
       match a with
+      | @own _ _ M IN r => @OwnM Σ (to_LURA M) (SUB M IN) r
       | owne E => OwnE n E
       | ownd D => OwnD n D
       | owni i p => @OwnI Σ Formulas _ n i p
@@ -114,57 +126,59 @@ Module Atoms.
 
   End INTERP.
 
-End Atoms.
+End Atom.
 
 Section WSAT.
 
-  Context `{Σ : GRA.t}.
+  Context `{σ : list PCMForSyntax.URA.t}.
+  Context `{Σ : PCM.GRA.t}.
+  Context `{SUB : forall M, In M σ -> PCM.GRA.inG (to_LURA M) Σ}.
   (* Context `{Interp : Base.InterpMeta}. *)
 
   (* Local Notation T := Base.t. *)
   (* Local Notation TSem := (@Base.sem Base.interp). *)
   (* Local Notation TSem := (Base.sem). *)
 
-  Local Notation typing := (@Syntax.Typ (@Atoms.t)).
-  Local Notation Formulas := (fun (n : index) => @Syntax.t (typing n) (@Atoms.t (typing n))).
-  (* Local Notation typing := (@Syntax.Typ T TSem (@Atoms.t T)). *)
-  (* Local Notation Formulas := (fun (n : index) => @Syntax.t T (typing n) (@Atoms.t T (typing n))). *)
+  Local Notation typing := (@Syntax.Typ (@Atom.t σ)).
+  Local Notation Formulas := (fun (n : index) => @Syntax.t (typing n) (@Atom.t σ (typing n))).
+  (* Local Notation typing := (@Syntax.Typ T TSem (@Atom.t T)). *)
+  (* Local Notation Formulas := (fun (n : index) => @Syntax.t T (typing n) (@Atom.t T (typing n))). *)
 
-  Context `{@GRA.inG (IInvSetRA Formulas) Σ}.
-  Context `{@GRA.inG (index ==> CoPset.t)%ra Σ}.
-  Context `{@GRA.inG (index ==> Gset.t)%ra Σ}.
+  Context `{@PCM.GRA.inG (IInvSetRA Formulas) Σ}.
+  Context `{@PCM.GRA.inG (PCM.URA.pointwise index PCM.CoPset.t) Σ}.
+  Context `{@PCM.GRA.inG (PCM.URA.pointwise index PCM.Gset.t) Σ}.
 
-  Local Notation AtomSem := (@Atoms.to_semantics Σ _ _ _).
-  Local Notation SynSem := (@Syntax.to_semantics Σ (@Atoms.t) AtomSem).
-  (* Local Notation AtomSem := (@Atoms.to_semantics Σ _ TSem _ _ _). *)
-  (* Local Notation SynSem := (@Syntax.to_semantics Σ _ TSem (@Atoms.t T) AtomSem). *)
+  Local Notation AtomSem := (@Atom.to_semantics σ Σ SUB _).
+  Local Notation SynSem := (@Syntax.to_semantics Σ (@Atom.t σ) AtomSem).
+  (* Local Notation AtomSem := (@Atom.to_semantics Σ _ TSem _ _ _). *)
+  (* Local Notation SynSem := (@Syntax.to_semantics Σ _ TSem (@Atom.t T) AtomSem). *)
 
-  Global Instance SynIISet : @IInvSet Σ Formulas := (@Syntax.IISet Σ (@Atoms.t) AtomSem).
-  (* Global Instance SynIISet : @IInvSet Σ Formulas := (@Syntax.IISet Σ _ TSem (@Atoms.t T) AtomSem). *)
+  Global Instance SynIISet : @IInvSet Σ Formulas := (@Syntax.IISet Σ (@Atom.t σ) AtomSem).
+  (* Global Instance SynIISet : @IInvSet Σ Formulas := (@Syntax.IISet Σ _ TSem (@Atom.t T) AtomSem). *)
 
 
-  Definition syn_inv_auth n (ps : gmap positive (Formulas n)) : @Atoms.t (typing n) :=
-    Atoms.syn_inv_auth_l (map_to_list ps).
-  (* Definition syn_inv_auth n (ps : gmap positive (Formulas n)) : @Atoms.t T (typing n) := *)
-  (*   Atoms.syn_inv_auth_l (map_to_list ps). *)
+  Definition syn_inv_auth n (ps : gmap positive (Formulas n)) : @Atom.t σ (typing n) :=
+    Atom.syn_inv_auth_l (map_to_list ps).
+  (* Definition syn_inv_auth n (ps : gmap positive (Formulas n)) : @Atom.t T (typing n) := *)
+  (*   Atom.syn_inv_auth_l (map_to_list ps). *)
 
   Lemma syn_inv_auth_iProp
         n ps
     :
-    Atoms.to_semantics n (syn_inv_auth n ps) = inv_auth n ps.
+    Atom.to_semantics n (syn_inv_auth n ps) = inv_auth n ps.
   Proof.
     ss. rewrite list_to_map_to_list. ss.
   Qed.
 
-  Import Atoms Syntax.
+  Import Atom Syntax.
 
   Definition syn_inv_satall_fun n : positive -> (Formulas n) -> (Formulas n) :=
     fun i p => or (sepconj p (atom (ownd {[i]}))) (atom (owne {[i]})).
   (* fun i p => Syntax.or (Syntax.sepconj p (Syntax.atom (ownd {[i]}))) (Syntax.atom (owne {[i]})). *)
 
   Definition syn_inv_satall n (ps : gmap positive (Formulas n)) : Formulas n :=
-    @star_gmap (@Atoms.t) n ps (syn_inv_satall_fun n).
-    (* @star_gmap _ TSem (@Atoms.t T) n ps (syn_inv_satall_fun n). *)
+    @star_gmap (@Atom.t σ) n ps (syn_inv_satall_fun n).
+    (* @star_gmap _ TSem (@Atom.t T) n ps (syn_inv_satall_fun n). *)
   (* @Syntax.star_gmap _ TSem (@t T) n ps (inv_satall_fun n). *)
 
 
@@ -287,7 +301,7 @@ End FUPD.
 
     Context `{TSem : T -> Type}.
 
-    Local Notation t := Atoms.t.
+    Local Notation t := Atom.t.
 
 
     Local Notation typing := (@Syntax.Typ T TSem t).
@@ -315,7 +329,7 @@ End FUPD.
 (*   Context `{T : Type}. *)
 (*     Context `{TSem : T -> Type}. *)
 
-(*     (* Atoms should not interpret arguments. *) *)
+(*     (* Atom should not interpret arguments. *) *)
 (*     Inductive As (V : @type T -> Type) : Type := *)
 (*       | owni (p : V formulaT) *)
 (*     . *)
@@ -425,7 +439,7 @@ End FUPD.
 (*     Context `{T : Type}. *)
 (*     Context `{TSem : T -> Type}. *)
 
-(*     (* Atoms should not interpret arguments. *) *)
+(*     (* Atom should not interpret arguments. *) *)
 (*     Inductive As (V : @type T -> Type) : Type := *)
 (*       | owni (p : V formulaT) *)
 (*     . *)
